examples/mutsum/MutFG.v
@@ -130,12 +130,9 @@ Then, we can just use SimModSem.adequacy_local_list. in this proof (FG23_correct
     ii.
     eapply ModSemLPair.mk with (wf:=top1) (le:=top2); ss.
     econs; [|econs; [|econs;ss]].
-    - init. unfold fun_to_src, cfun, body_to_src, mainBody, interp_hCallE_src, compose.
-      admit "ez; interp_red. steps. interp_red. steps. interp_red. steps".
-    - init. unfold fun_to_src, cfun, body_to_src, mainBody, interp_hCallE_src.
-      admit "ez; interp_red. steps. force_l. eexists. steps".
-    - init. unfold fun_to_src, cfun, body_to_src, mainBody, interp_hCallE_src.
-      admit "ez; interp_red. steps. force_l. eexists. steps".
+    - admit "SimModSemL".
+    - admit "SimModSemL".
+    - admit "SimModSemL".
   Qed.
 
   Theorem FG_correct:
